{
 "cells": [
  {
   "cell_type": "markdown",
   "metadata": {},
   "source": [
    "# Functions \n",
    "\n",
    "Functions can only have one output for any given input.  So $ \\pm\\sqrt{x} $ is Not a function, cus it has two outputs.\n",
    "\n",
    "*Domain* - Inputs.  *Range* - Outputs.\n",
    "\n",
    "## Rational Function\n",
    "\n",
    "$$\n",
    "\\frac{f(x)}{g(x)}\n",
    "$$\n"
   ]
  },
  {
   "cell_type": "markdown",
   "metadata": {},
   "source": [
    "# Inequalities\n",
    "\n",
    "You can apply a **monotonically** increasing function to both sides without changing the inequality. If you apply a monotonically decreasing function to both sides you need to reverse the inequality.\n",
    "\n",
    "**Multiplication/Division**\n",
    "\n",
    "If $a \\leq b$ and $ c > 0: ac\\leq bc$\n",
    "\n",
    "If $a \\leq b$ and $ c < 0: ac\\geq bc$\n",
    "\n",
    "**Additive Inverse**\n",
    "\n",
    "If $a \\leq b$, then $-a \\geq -b$\n",
    "\n",
    "**Multiplicative Inverse**\n",
    "If $0 < a \\leq b$ then $\\frac{1}{a} \\geq \\frac{1}{b} > 0$.\n",
    "\n",
    "If $a \\leq b < 0$ then $ 0 > \\frac{1}{a} \\geq \\frac{1}{b} $.\n",
    "\n",
    "If $a < 0 < b$ then $\\frac{1}{a} < 0 < \\frac{1}{b}$.\n",
    "\n",
    "## Solving Polynomial Inequalities\n",
    "\n",
    "The roots are the only places where the polynomial can change sign, so thats where we look for inequalities.  Odd exponents can switch sign, even exponents will always be positive.\n",
    "\n",
    "\n",
    "## Solving Rational Function Inequalities\n",
    "\n",
    "Of the form\n",
    "\n",
    "$$\n",
    "\\frac{f(x)}{g(x)} < 0\n",
    "$$\n",
    "\n",
    "Or any other form of ineqaulity like greater than equal, etc.  With functions like these, you need to consider both roots and vertical asymptotes -- those are where sign switches can occur.  Apply da wavy curve method from there to get your inequality:\n",
    "\n",
    "https://brilliant.org/wiki/wavy-curve-method/\n",
    "\n"
   ]
  },
  {
   "cell_type": "markdown",
   "metadata": {},
   "source": [
    "# Absolute Value\n",
    "\n",
    "Geometrically we can think of absolute value as distance from 0 on the number line.  \n",
    "\n",
    "Mathematically we can think of it as\n",
    "\n",
    "$$\n",
    "f(x) =\n",
    "\\begin{cases}\n",
    "p ~&\\text{ if }~ p \\geq 0 \\\\\n",
    "-p ~&\\text{ if }~ p < 0 \\\\\n",
    "\\end{cases}\n",
    "$$\n",
    "\n"
   ]
  },
  {
   "cell_type": "markdown",
   "metadata": {},
   "source": [
    "\n",
    "# Rationalizing the denominator\n",
    "\n",
    "Rationalizing the denominator is a convention, but rationalizing denominator or numerator can sometimes help solve encapsulating problems like limits.\n",
    "\n",
    "$$ (\\frac{1}{\\sqrt{2}})(\\frac{\\sqrt{2}}{\\sqrt{2}}) = \\frac{\\sqrt{2}}{2}$$\n",
    "\n",
    "$$ (\\frac{12}{2-\\sqrt{5}})(\\frac{2 + \\sqrt{5}}{2 + \\sqrt{5}}) = -24 - 2\\sqrt{5}$$\n",
    "\n",
    "# Exponent Rules\n",
    "\n",
    "**Power of a Power**: $$(b^x)^y = b^{xy}$$\n",
    "**Multiplying Exponents**: $$ b^{x}b^{y} = b^{x+y} $$\n",
    "**Dividing Exponents**: $$ \\frac{b^x}{b^y} = b^{x-y} $$\n",
    "**Distribute Power of Products**: $$ (ab)^x = a^{x}b^x $$\n",
    "\n",
    "# Log rules\n",
    "\n",
    "Will prove each one in terms of previous Exponent and Log rules.\n",
    "\n",
    "**Log Product Rule**: $$ \\log_{b}(MN) = \\log_{b}(M) + \\log_{b}(N) $$\n",
    "Proof:\n",
    "$$\n",
    "\\begin{align*}\n",
    "& x = \\log_{b}(MN) \\\\\n",
    "& y =  \\log_{b}(M) \\\\ \n",
    "& z = \\log_{b}(N) \\\\\n",
    "& b^y = M \\\\\n",
    "& b^z = N \\\\\n",
    "& b^x = MN = b^{y}b^{z} = b^{y + z} \\quad\\text{Multiplying Exponents} \\\\\n",
    "& x = y + z \\\\\n",
    "& \\log_{b}(MN) = \\log_{b}(M) + \\log_{b}(N)\n",
    "\\end{align*}\n",
    "$$\n",
    "\n",
    "**Log Quotient Rule**: $$ \\log_{b}(M/N) = \\log_{b}(M) - \\log_{b}(N) $$\n",
    "Proof:\n",
    "$$\n",
    "\\begin{align*}\n",
    "& x = \\log_{b}(M/N) \\\\\n",
    "& y =  \\log_{b}(M) \\\\ \n",
    "& z = \\log_{b}(N) \\\\\n",
    "& b^y = M \\\\\n",
    "& b^z = N \\\\\n",
    "& b^x = M/N = \\frac{b^y}{b^z} = b^{y - z} \\quad\\text{Dividing Exponents} \\\\\n",
    "& x = y - z \\\\\n",
    "& \\log_{b}(M/N) = \\log_{b}(M) - \\log_{b}(N)\n",
    "\\end{align*}\n",
    "$$\n",
    "\n",
    "**Log Power Rule**: $$ \\log_{b}(M^p) = p\\log_{b}(M) $$\n",
    "Proof:\n",
    "$$\n",
    "\\begin{align*}\n",
    "& x = \\log_{b}(M^p) \\\\\n",
    "& y = \\log_{b}(M) \\\\\n",
    "& b^y = M \\\\\n",
    "& b^x = M^p \\\\\n",
    "& b^x = (b^y)^p \\\\\n",
    "& b^x = b^{yp} \\quad\\text{Power of a Power} \\\\\n",
    "& x = py \\\\\n",
    "& \\log_{b}(M^p) = p\\log_{b}(M) \\\\\n",
    "\\end{align*}\n",
    "$$\n",
    "\n",
    "**Change of Base Rule**: $$ \\log_{a}(x) = \\frac{\\log_{b}(x)}{\\log_{b}(a)} $$\n",
    "Proof:\n",
    "$$\n",
    "\\begin{align*}\n",
    "& a^y = x \\\\\n",
    "& \\log_{b}(a^y) = \\log_{b}(x) \\\\\n",
    "& y\\log_{b}(a) = \\log_{b}(x) \\quad\\text{Log Power Rule} \\\\\n",
    "& y = \\frac{\\log_{b}(x)}{\\log_{b}(a)} \\\\\n",
    "& \\log_{a}(x) = \\frac{\\log_{b}(x)}{\\log_{b}(a)} \n",
    "\\end{align*}\n",
    "$$"
   ]
  },
  {
   "cell_type": "code",
   "execution_count": null,
   "metadata": {},
   "outputs": [],
   "source": [
    "5 ** 10 # 5^10\n",
    "\n",
    "# math.log(x, [base=e])\n",
    "math.log(4, 2) # Log 4 base 2.\n",
    "math.log(10) # Log 10 base e"
   ]
  },
  {
   "cell_type": "markdown",
   "metadata": {},
   "source": [
    "# Polynomials\n",
    "\n",
    "## Defining Terms\n",
    "\n",
    "*Polynomial* One of those equations with coefficients, variables, and non negative exponentiation combined with addition/multiplication/etc.\n",
    "\n",
    "*Quadratic* functions are polynomials of degree 2.\n",
    "\n",
    "*Parabola* - graph of a quadratic.  They have those open face shapes and point up or down. \n",
    "\n",
    "One definition of a parabola is that it's the set of points which are equidistant from a Focus (a point) and a Directrix (Line).\n",
    "\n",
    "Forms of equations for a parabola with examples:\n",
    "\n",
    "- *Standard Form* - $ 3x^2 + 12x - 15 $\n",
    "- *Factored Form* - $ 3(x-1)(x+5) $\n",
    "- *Vertex Form* - $ 3(x+2)^2 - 27 $\n",
    "\n",
    "Abstraction of vertex form we learned in Geometry lesson:\n",
    "$$ y = a(x-h)^2 + k $$\n",
    "$$ x = a(y-k)^2 + h $$\n",
    "\n",
    "Where $ (h, k) $ is the *Vertex* of the parabola. That Vertex is either the top or the bottom.\n",
    "\n",
    "Aha! Just noticed the Vertex and the Root (derived from factored form) could be same, if there's no constant term.\n",
    "\n",
    "*Monic* quadratics are expressions where the leading coefficient ($a$) is equal to $1$.\n",
    "\n",
    "## Fundamental Theorem of Algebra\n",
    "\n",
    "Any every polynomial equation of degree $ n $ with complex number coefficients has $ n $ roots, or solutions, in the complex numbers.\n",
    "\n",
    "Explanation of why roots can count twice, such as in $x^2$  which has a repeating 0 root. https://math.stackexchange.com/a/1131546/49487\n",
    "\n",
    "Proving it: requires some pretty advanced math, worth doing _after_ getting good with calc.\n",
    "\n",
    "## Completing the Square\n",
    "\n",
    "Completing the square works on any quadratic, and is actually the proof basis of the Quadratic Formula.\n",
    "\n",
    "Make sure to divide out coefficient $a$ before completing the square.  Then just add a constant factor thats the square of half coefficient $b$ to do your squaring proper.\n",
    "\n",
    "Completing the square works cus it lets you take a square root of both sides to eliminate the 2nd degree factor.\n",
    "\n",
    "Make sure that when you complete the square and do the final square root step, that you remember this produces a $ \\pm $ value.\n",
    "\n",
    "## Quadratic Formula\n",
    "\n",
    "$ x=\\frac{-b\\pm\\sqrt{b^2-4ac}}{2a} $\n",
    "\n",
    "The discriminant is the part of the quadratic formula underneath the square root symbol: $ b^2-4ac $. The discriminant tells us whether there are two solutions, one solution, or no solutions.\n",
    "\n",
    "* Positive Discriminant - $ b^2 - 4ac > 0 $ - 2 real roots\n",
    "* Zero Discriminant - $ b^2 - 4ac = 0 $ - 1 repeated real 0 root.\n",
    "* Negative Discriminant - $ b^2 - 4ac < 0 $ - 2 imaginary roots.\n",
    "\n",
    "### Proof of Quadratic Formula using Completing the Square\n",
    "\n",
    "$$\n",
    "\\begin{align*}\n",
    "ax^2 + bx + c = 0 \\\\\n",
    "x^2 + \\frac{bx}{a} + \\frac{c}{a} = 0 \\\\\n",
    "x^2 + \\frac{bx}{a} + \\frac{c}{a} + ((\\frac{b}{2a})^2 - \\frac{c}{a}) = ((\\frac{b}{2a})^2 - \\frac{c}{a}) \\\\\n",
    "x^2 + \\frac{bx}{a} + (\\frac{b}{2a})^2  = (\\frac{b}{2a})^2 - \\frac{c}{a} \\\\\n",
    "(x + \\frac{b}{2a})^2 = (\\frac{b}{2a})^2 - \\frac{c}{a} \\quad\\text{Complete the Square} \\\\\n",
    "(x + \\frac{b}{2a})^2 = \\frac{b^2}{4a^2} - \\frac{c}{a} \\\\\n",
    "(x + \\frac{b}{2a})^2 = \\frac{b^2 - 4ac}{4a^2} \\\\\n",
    "x + \\frac{b}{2a} = \\pm\\sqrt{\\frac{b^2 - 4ac}{4a^2}} \\\\\n",
    "x + \\frac{b}{2a} = \\frac{\\pm\\sqrt{b^2 - 4ac}}{2a} \\\\\n",
    "x = \\frac{-b\\pm\\sqrt{b^2 - 4ac - b}}{2a}\n",
    "\\end{align*}\n",
    "$$\n",
    "\n",
    "## Binomial Theorem\n",
    "\n",
    "$$ (a+b)^n = \\sum_{k=0}^{n}\\binom{n}{k}a^{n-k}b^k $$\n",
    "\n",
    "We know that this is true for $n = 1$, so we can prove it by induction for all positive numbers. So we seek to prove that\n",
    "\n",
    "$$ \n",
    "\\begin{align}\n",
    "& (a+b)^{n+1} = \\sum_{k=0}^{n+1}\\binom{n+1}{k}a^{n+1-k}b^k \\\\\n",
    "& (a + b)(a+b)^n \\\\\n",
    "& (a + b)\\sum_{k=0}^{n}\\binom{n}{k}a^{n-k}b^k \\quad\\text {Induction} \\\\\n",
    "& \\left(\\sum_{k=0}^{n}\\binom{n}{k}a^{n-k + 1}b^k\\right) + \\left(\\sum_{k=0}^{n}\\binom{n}{k}a^{n-k}b^{k+1}\\right) \\\\\n",
    "& \\left(\\binom{n}{0}a^{n+1}b^0 + \\sum_{k=1}^{n}\\binom{n}{k}a^{n-k + 1}b^k\\right) + \\left(\\sum_{k=1}^{n+1}\\binom{n}{k-1}a^{n-k+1}b^{k}\\right) \\\\\n",
    "& \\left(a^{n+1} + \\sum_{k=1}^{n}\\binom{n}{k}a^{n-k + 1}b^k\\right) + \\left(\\binom{n}{n}a^{0}b^{n+1} + \\sum_{k=1}^{n}\\binom{n}{k-1}a^{n-k+1}b^{k}\\right) \\\\\n",
    "& a^{n+1} + b^{n+1} + \\sum_{k=1}^{n}\\binom{n}{k}a^{n-k + 1}b^k + \\sum_{k=1}^{n}\\binom{n}{k-1}a^{n-k+1}b^{k} \\\\\n",
    "& a^{n+1} + b^{n+1} + \\sum_{k=1}^{n}\\binom{n+1}{k}a^{n-k + 1}b^k \\quad\\text {Pascal's Identity} \\\\\n",
    "& \\binom{n+1}{0} a^{n-0+1}b^0 + \\binom{n+1}{n+1}a^{n-(n+1)+1}b^{n+1} + \\sum_{k=1}^{n}\\binom{n+1}{k}a^{n-k + 1}b^k \\\\\n",
    "& \\sum_{k=0}^{n+1}\\binom{n+1}{k}a^{n-k + 1}b^k \\\\\n",
    "\\end{align}\n",
    "$$ "
   ]
  },
  {
   "cell_type": "markdown",
   "metadata": {},
   "source": [
    "# Even vs Odd Functions\n",
    "\n",
    "*Even functions* can be flipped over the y-axis, *Odd functions* have to be flipped over x and y axis.  \n",
    "\n",
    "**Even function**:\n",
    "$$ f(x) = f(-x) $$\n",
    "\n",
    "**Odd function**\n",
    "$$ f(x) = -f(-x) $$\n",
    "\n",
    "Only 0 can be both even and odd (e.g. $f(x) = 0$).  Thing can be neithern (e.g. $(x-2)^2$) depending on whether those equalities hold or not.. Simplest way to check function for even/odd is just to plugin x.  Same value means even, every term being _opposite_ implies odd."
   ]
  }
 ],
 "metadata": {
  "interpreter": {
   "hash": "949777d72b0d2535278d3dc13498b2535136f6dfe0678499012e853ee9abcab1"
  },
  "kernelspec": {
   "display_name": "Python 3 (ipykernel)",
   "language": "python",
   "name": "python3"
  },
  "language_info": {
   "codemirror_mode": {
    "name": "ipython",
    "version": 3
   },
   "file_extension": ".py",
   "mimetype": "text/x-python",
   "name": "python",
   "nbconvert_exporter": "python",
   "pygments_lexer": "ipython3",
   "version": "3.9.2"
  }
 },
 "nbformat": 4,
 "nbformat_minor": 4
}
